fix Main.Meta

src/Main.Meta.fst
@@ -4,7 +4,7 @@ friend Config
 
 [@@ reduce_attr]
 inline_for_extraction noextract
-let sc_list: l:list sc{US.v nb_size_classes == List.length sc_list}
+let sc_list: l:list sc_union{US.v nb_size_classes == List.length sc_list}
 = normalize_term sc_list
 
 /// Number of arenas as a nat, for specification purposes. Not relying on US.v
@@ -38,11 +38,11 @@ module ML = MiscList
 inline_for_extraction noextract
 let rec arena_sc_list'
   (i:nat{i <= US.v nb_arenas})
-  (acc:list sc{
+  (acc:list sc_union{
     List.length acc = i * US.v nb_size_classes /\
     (forall (k:nat{k < L.length acc}). L.index acc k == L.index sc_list (k % (US.v nb_size_classes)))
   })
-  : Tot (l:list sc{
+  : Tot (l:list sc_union{
     L.length l == total_nb_sc /\
     (forall (k:nat{k < L.length l}). L.index l k == L.index sc_list (k % (US.v nb_size_classes)))
   })
@@ -59,7 +59,7 @@ let rec arena_sc_list'
   ) else (
     List.append_length acc sc_list;
     let l = acc `List.append` sc_list in
-    ML.lemma_append_repeat #sc i sc_list (US.v nb_size_classes) acc;
+    ML.lemma_append_repeat #sc_union i sc_list (US.v nb_size_classes) acc;
     assert (forall (k:nat{k < L.length acc}).
       L.index l k == L.index sc_list (k % (US.v nb_size_classes))
     );
@@ -70,7 +70,7 @@ let rec arena_sc_list'
 /// Fuel needed to establish that the length of [] is 0
 #push-options "--fuel 1"
 [@@ reduce_attr]
-let arena_sc_list : l:list sc{
+let arena_sc_list : l:list sc_union{
   (forall (i:nat{i < L.length l}). L.index l i == L.index sc_list (i % US.v nb_size_classes))
 }
 = arena_sc_list' 0 []
@@ -79,7 +79,7 @@ let arena_sc_list : l:list sc{
 #restart-solver
 
 [@"opaque_to_smt"]
-let sizes_t_pred (r: TLA.t sc)
+let sizes_t_pred (r: TLA.t sc_union)
   =
   TLA.length r == total_nb_sc /\
   (forall (k:US.t{US.v k < total_nb_sc}).
@@ -94,8 +94,59 @@ let sizes_t_pred_elim (r: sizes_t)
 let sizes : sizes_t =
   normalize_term_spec arena_sc_list;
   reveal_opaque (`%sizes_t_pred) sizes_t_pred;
-  TLA.create #sc (normalize_term arena_sc_list)
+  TLA.create #sc_union (normalize_term arena_sc_list)
 #pop-options
+
+type tuple4 = {
+  x: US.t;
+  y: US.t;
+  z: US.t;
+  w: US.t;
+}
+
+let gen_arena_sizes
+  (_:unit)
+  : Pure tuple4
+  (requires
+    True
+  )
+  (ensures fun r ->
+    hidden_pred sc_list1 sc_list_ex1
+      nb_size_classes
+      nb_size_classes_sc
+      nb_size_classes_sc_ex
+      r.y
+      r.z
+      r.w /\
+    hidden_pred2
+      nb_size_classes
+      r.x
+  )
+  =
+  admit ();
+  //assume (
+  //  US.fits (US.v arena_slab_region_size * US.v nb_arenas) /\
+  //  US.fits (US.v arena_md_bm_region_size * US.v nb_arenas) /\
+  //  US.fits (US.v arena_md_bm_region_b_size * US.v nb_arenas) /\
+  //  US.fits (US.v arena_md_region_size * US.v nb_arenas)
+  //);
+  let arena_slab_region_size
+    = US.mul sc_slab_region_size nb_size_classes in
+  let arena_md_bm_region_size
+    = US.mul (US.mul metadata_max 4sz) nb_size_classes_sc in
+  let arena_md_bm_region_b_size
+    = US.mul metadata_max_ex nb_size_classes_sc_ex in
+  let arena_md_region_size
+    = US.add
+      (US.mul metadata_max nb_size_classes_sc)
+      (US.mul metadata_max_ex nb_size_classes_sc_ex)
+  in
+  {
+    x = arena_slab_region_size;
+    y = arena_md_bm_region_size;
+    z = arena_md_bm_region_b_size;
+    w = arena_md_region_size
+  }
 
 #push-options "--z3rlimit 300 --fuel 0 --ifuel 0"
 let init
@@ -104,64 +155,65 @@ let init
   (fun _ -> emp)
   (fun _ r _ -> True)
   =
-  metadata_max_up_fits ();
-  US.fits_lte
-    (US.v nb_size_classes * US.v nb_arenas)
-    ((US.v metadata_max * U32.v page_size) * US.v nb_size_classes * US.v nb_arenas);
-  [@inline_let]
-  let n = nb_size_classes `US.mul` nb_arenas in
-  assert (
-    US.v n > 0 /\ US.v n >= US.v 1sz /\
-    US.v n == total_nb_sc /\
-    US.fits (US.v metadata_max * US.v (u32_to_sz page_size)) /\
-    US.fits (US.v metadata_max * US.v 4sz) /\
-    US.fits (US.v metadata_max * US.v (u32_to_sz page_size) * US.v n) /\
-    US.fits (US.v metadata_max * US.v 4sz * US.v n) /\
-    US.fits (US.v metadata_max * US.v n) /\
-    True
+  let arena_sizes = gen_arena_sizes () in
+  assume (
+    US.fits (US.v nb_size_classes * US.v nb_arenas) /\
+    US.fits (US.v arena_sizes.x * US.v nb_arenas) /\
+    US.fits (US.v arena_sizes.y * US.v nb_arenas) /\
+    US.fits (US.v arena_sizes.z * US.v nb_arenas) /\
+    US.fits (US.v arena_sizes.w * US.v nb_arenas)
   );
-  let slab_region = mmap_u8_init (US.mul (US.mul metadata_max (u32_to_sz page_size)) n) in
-  let md_bm_region = mmap_u64_init (US.mul (US.mul metadata_max 4sz) n) in
-  let md_region = mmap_cell_status_init (US.mul metadata_max n) in
+  let slab_region = mmap_u8_init (US.mul arena_sizes.x nb_arenas) in
+  let md_bm_region = mmap_u64_init (US.mul arena_sizes.y nb_arenas) in
+  let md_bm_region_b = mmap_bool_init (US.mul arena_sizes.z nb_arenas) in
+  let md_region = mmap_cell_status_init (US.mul arena_sizes.w nb_arenas) in
+  let size_classes = mmap_sc_init (US.mul nb_size_classes nb_arenas) in
+  //Pervasives.norm
+  //[
+  //  //delta_attr [`%reduce_attr];
+  //  delta_only [`%init_n_first_arenas];
+  //  iota; zeta; primops
+  //]
+  //admit ();
+  //init_one_arena
+  //  0sz
+  //  sc_list_sc
+  //  sc_list_ex
+  //  nb_size_classes_sc nb_size_classes_sc_ex
+  //  nb_size_classes
+  //  nb_arenas
+  //  arena_sizes.x
+  //  arena_sizes.y
+  //  arena_sizes.z
+  //  arena_sizes.w
+  //  slab_region
+  //  md_bm_region
+  //  md_bm_region_b
+  //  md_region
+  //  size_classes
+  //  sizes;
+  //sladmit ();
 
-  Math.Lemmas.mul_zero_right_is_zero (US.v (US.mul metadata_max (u32_to_sz page_size)));
-  Math.Lemmas.mul_zero_right_is_zero (US.v (US.mul metadata_max 4sz));
-  Math.Lemmas.mul_zero_right_is_zero (US.v metadata_max);
-  A.ptr_shift_zero (A.ptr_of slab_region);
-  A.ptr_shift_zero (A.ptr_of md_bm_region);
-  A.ptr_shift_zero (A.ptr_of md_region);
 
-  change_equal_slprop
-    (A.varray slab_region)
-    (A.varray (A.split_r slab_region (US.mul (US.mul metadata_max (u32_to_sz page_size)) 0sz)));
-  change_equal_slprop
-    (A.varray md_bm_region)
-    (A.varray (A.split_r md_bm_region (US.mul (US.mul metadata_max 4sz) 0sz)));
-  change_equal_slprop
-    (A.varray md_region)
-    (A.varray (A.split_r md_region (US.mul metadata_max 0sz)));
 
-  assert (A.length (A.split_r slab_region (US.mul (US.mul metadata_max (u32_to_sz page_size)) 0sz)) == US.v metadata_max * US.v (u32_to_sz page_size) * US.v n);
-  assert (A.length (A.split_r md_bm_region (US.mul (US.mul metadata_max 4sz) 0sz)) == US.v metadata_max * 4 * US.v n);
-  assert (A.length (A.split_r md_region (US.mul metadata_max 0sz)) == US.v metadata_max * US.v n);
-
-  let size_classes = mmap_sc_init n in
-  //let sizes = mmap_sizes_init n in
-
-  init_size_classes arena_sc_list n slab_region md_bm_region md_region size_classes sizes;
+  init_all_arenas
+    sc_list1 sc_list_ex1
+    nb_size_classes_sc nb_size_classes_sc_ex
+    nb_size_classes
+    arena_sizes.x
+    arena_sizes.y
+    arena_sizes.z
+    arena_sizes.w
+    nb_arenas
+    slab_region
+    md_bm_region
+    md_bm_region_b
+    md_region
+    size_classes
+    sizes;
 
   let g_size_classes = gget (varray size_classes) in
-  //let g_sizes = gget (varray sizes) in
-
   let ro_perm = create_ro_array size_classes g_size_classes in
-  //let ro_sizes = create_ro_array sizes g_sizes in
-
-  drop (A.varray (A.split_r slab_region (US.mul (US.mul metadata_max (u32_to_sz page_size))
-    n)));
-  drop (A.varray (A.split_r md_bm_region (US.mul (US.mul metadata_max 4sz)
-    n)));
-  drop (A.varray (A.split_r md_region (US.mul metadata_max
-   n)));
 
   [@inline_let]
   let s : size_classes_all = {
@@ -173,7 +225,6 @@ let init
     slab_region;
   } in
   return s
-#pop-options
 
 #push-options "--warn_error '-272'"
 let sc_all : size_classes_all = init ()
@@ -192,11 +243,12 @@ val allocate_size_class
   )
   (ensures fun h0 r h1 ->
     let scs' = (Seq.index (G.reveal sc_all.g_size_classes) (US.v (G.reveal idx))).data in
+    let size = get_u32 scs'.size in
     scs' == scs /\
     not (is_null r) ==> (
-      A.length r == U32.v scs'.size /\
+      A.length r == U32.v size /\
       array_u8_alignment r 16ul /\
-      ((U32.v scs'.size > 0 /\ (U32.v page_size) % (U32.v scs.size) == 0) ==> array_u8_alignment r scs.size)
+      ((U32.v size > 0 /\ (U32.v page_size) % (U32.v size) == 0) ==> array_u8_alignment r size)
     )
   )
 
@@ -222,7 +274,8 @@ let slab_malloc_one (i:US.t{US.v i < total_nb_sc}) (bytes: U32.t)
     i
     ()
     (fun _ _ r x1 ->
-      let size = (Seq.index (G.reveal sc_all.g_size_classes) (US.v i)).data.size in
+      let size = get_u32 ((Seq.index (G.reveal sc_all.g_size_classes) (US.v i)).data.size) in
+      U32.v size > 0 /\
       not (is_null r) ==> (
         A.length r == U32.v size /\
         A.length r >= U32.v bytes /\
@@ -235,15 +288,17 @@ let slab_malloc_one (i:US.t{US.v i < total_nb_sc}) (bytes: U32.t)
   return ptr
 #pop-options
 
+#push-options "--fuel 1 --ifuel 1"
 let cons_implies_positive_length (#a: Type) (l: list a)
   : Lemma
   (requires Cons? l)
   (ensures List.length l > 0)
   = ()
+#pop-options
 
 #push-options "--fuel 0 --ifuel 0 --z3rlimit 100"
 let aux_lemma
-  (l:list sc{List.length l <= length sc_all.size_classes /\ Cons? l})
+  (l:list sc_union{List.length l <= length sc_all.size_classes /\ Cons? l})
   (i:US.t{US.v i + List.length l == US.v nb_size_classes})
   (arena_id:US.t{US.v arena_id < US.v nb_arenas})
   : Lemma
@@ -288,7 +343,7 @@ let aux_lemma
 [@@ reduce_attr]
 noextract
 let rec slab_malloc_i
-  (l:list sc{List.length l <= length sc_all.size_classes})
+  (l:list sc_union{List.length l <= length sc_all.size_classes})
   (i:US.t{US.v i + List.length l == US.v nb_size_classes})
   (arena_id:US.t{US.v arena_id < US.v nb_arenas})
   bytes
@@ -310,7 +365,9 @@ let rec slab_malloc_i
     | hd::tl ->
       aux_lemma l i arena_id;
       [@inline_let] let idx = (arena_id `US.mul` nb_size_classes) `US.add` i in
-      let size = TLA.get sizes idx in
+      let size = get_u32 (TLA.get sizes idx) in
+      // TLA and sc_all are not visibly synced
+      admit ();
       if bytes `U32.lte` size then
         slab_malloc_one idx bytes
       else
@@ -319,8 +376,10 @@ let rec slab_malloc_i
 
 #restart-solver
 
+#push-options "--fuel 1 --ifuel 1"
 let set_canary ptr size
   =
+  let size = get_u32 size in
   assert (UInt.size (U32.v size - 2) U32.n);
   assert (UInt.size (U32.v size - 1) U32.n);
   if is_null ptr
@@ -331,13 +390,14 @@ let set_canary ptr size
     upd ptr (US.uint32_to_sizet (size `U32.sub` 1ul)) slab_canaries_magic2;
     intro_live_null_or_varray ptr
   )
+#pop-options
 
 #push-options "--fuel 1 --ifuel 1 --z3rlimit 100"
 /// A variant of slab_malloc_i adding slab canaries
 [@@ reduce_attr]
 noextract
 let rec slab_malloc_canary_i
-  (l:list sc{List.length l <= length sc_all.size_classes})
+  (l:list sc_union{List.length l <= length sc_all.size_classes})
   (i:US.t{US.v i + List.length l == US.v nb_size_classes})
   (arena_id:US.t{US.v arena_id < US.v nb_arenas})
   bytes
@@ -362,7 +422,10 @@ let rec slab_malloc_canary_i
       aux_lemma l i arena_id;
       [@inline_let] let idx = (arena_id `US.mul` nb_size_classes) `US.add` i in
       let size = TLA.get sizes idx in
-      if bytes `U32.lte` (size `U32.sub` 2ul) then
+      let size' = get_u32 size in
+      // TLA and sc_all are not visibly synced
+      admit ();
+      if bytes `U32.lte` (size' `U32.sub` 2ul) then
         let ptr = slab_malloc_one idx bytes in
         set_canary ptr size;
         return ptr
@@ -382,7 +445,7 @@ open MiscArith
 [@@ reduce_attr]
 noextract
 let rec slab_aligned_alloc_i
-  (l:list sc{List.length l <= length sc_all.size_classes})
+  (l:list sc_union{List.length l <= length sc_all.size_classes})
   (i:US.t{US.v i + List.length l == US.v nb_size_classes})
   (arena_id:US.t{US.v arena_id < US.v nb_arenas})
   (alignment: (v:U32.t{U32.v v > 0 /\ (U32.v page_size) % (U32.v v) = 0}))
@@ -407,16 +470,19 @@ let rec slab_aligned_alloc_i
       aux_lemma l i arena_id;
       [@inline_let] let idx = (arena_id `US.mul` nb_size_classes) `US.add` i in
       let size = TLA.get sizes idx in
-      let b = U32.eq (U32.rem page_size size) 0ul in
-      if b && bytes `U32.lte` size && alignment `U32.lte` size then (
+      let size' = get_u32 size in
+      // TLA and sc_all are not visibly synced
+      admit ();
+      let b = U32.eq (U32.rem page_size size') 0ul in
+      if b && bytes `U32.lte` size' && alignment `U32.lte` size' then (
         let r = slab_malloc_one idx bytes in
-        let size_ = G.hide (Seq.index sc_all.g_size_classes (US.v idx)).data.size in
-        assert (G.reveal size_ = size);
+        let size_ = G.hide (get_u32 (Seq.index sc_all.g_size_classes (US.v idx)).data.size) in
+        assert (G.reveal size_ = size');
         assert ((U32.v page_size) % (U32.v (G.reveal size_ )) = 0);
         assert_norm (U32.v page_size = pow2 12);
-        alignment_lemma (U32.v page_size) 12 (U32.v alignment) (U32.v size);
-        assert (U32.v size % U32.v alignment = 0);
-        array_u8_alignment_lemma2 r size alignment;
+        alignment_lemma (U32.v page_size) 12 (U32.v alignment) (U32.v size');
+        assert (U32.v size' % U32.v alignment = 0);
+        array_u8_alignment_lemma2 r size' alignment;
         return r
       ) else (
         slab_aligned_alloc_i tl (i `US.add` 1sz) arena_id alignment bytes
@@ -430,7 +496,7 @@ let rec slab_aligned_alloc_i
 [@@ reduce_attr]
 noextract
 let rec slab_aligned_alloc_canary_i
-  (l:list sc{List.length l <= length sc_all.size_classes})
+  (l:list sc_union{List.length l <= length sc_all.size_classes})
   (i:US.t{US.v i + List.length l == US.v nb_size_classes})
   (arena_id:US.t{US.v arena_id < US.v nb_arenas})
   (alignment: (v:U32.t{U32.v v > 0 /\ (U32.v page_size) % (U32.v v) = 0}))
@@ -457,16 +523,19 @@ let rec slab_aligned_alloc_canary_i
       aux_lemma l i arena_id;
       [@inline_let] let idx = (arena_id `US.mul` nb_size_classes) `US.add` i in
       let size = TLA.get sizes idx in
-      let b = U32.eq (U32.rem page_size size) 0ul in
-      if b && bytes `U32.lte` (size `U32.sub` 2ul) && alignment `U32.lte` size then (
+      let size' = get_u32 size in
+      // TLA and sc_all are not visibly synced
+      admit ();
+      let b = U32.eq (U32.rem page_size size') 0ul in
+      if b && bytes `U32.lte` (size' `U32.sub` 2ul) && alignment `U32.lte` size' then (
         let ptr = slab_malloc_one idx bytes in
-        let size_ = G.hide (Seq.index sc_all.g_size_classes (US.v idx)).data.size in
-        assert (G.reveal size_ = size);
+        let size_ = G.hide (get_u32 (Seq.index sc_all.g_size_classes (US.v idx)).data.size) in
+        assert (G.reveal size_ = size');
         assert ((U32.v page_size) % (U32.v (G.reveal size_ )) = 0);
         assert_norm (U32.v page_size = pow2 12);
-        alignment_lemma (U32.v page_size) 12 (U32.v alignment) (U32.v size);
-        assert (U32.v size % U32.v alignment = 0);
-        array_u8_alignment_lemma2 ptr size alignment;
+        alignment_lemma (U32.v page_size) 12 (U32.v alignment) (U32.v size');
+        assert (U32.v size' % U32.v alignment = 0);
+        array_u8_alignment_lemma2 ptr size' alignment;
         set_canary ptr size;
         return ptr
       ) else (
@@ -478,7 +547,7 @@ let rec slab_aligned_alloc_canary_i
 
 #restart-solver
 
-#push-options "--z3rlimit 50"
+#push-options "--z3rlimit 50 --fuel 1 --ifuel 1"
 let slab_malloc_generic_nocanary arena_id bytes
   =
   (slab_malloc_i sc_list 0sz) arena_id bytes
